---
title: Concrete Mathematics, Chapter 1, warmups
---

## Exercise 1:

The demo doesn't cover one of the base cases. The case n = 1 is fine, but it is
missing n = 2, since to talk about a "middle horse" as it does during the
inductive step, there must be at least three horses, so we haven't established
anything for the case n = 2.

## Exercise 2:

If we have no disks, we do no moves, so $X_0 = 0$.
Playing a bit gives us the following initial values:
$X_1 = 2, X_2 = 8, X_3 = 26$
It is harder to notice from the values alone, but manually following the steps
gives us the following ideas:

After half the steps we built the tower in the middle peg (not relevant, but
worth noting).  To be able to move the nth (bottom) disc to the middle peg, we
need to build the tower $T_{n-1}$ of size (n-1) on B. Then we move
$T_{n-1}$ back to A, move the bottom disc to B, and finally move $T_{n-1}$ back
to A. In summary, the steps needed to move the tower of size n from A to B are
$X_n = 3X_{n-1}+2$

To find a closed form, we define $U_n = X_n + 1$, so that we can eliminate the
$(+2)$ from the equation.

$$
\begin{aligned}
U_n&= X_n + 1 \\
&=(3X_{n-1}+2) + 1 = (3(U_{n-1}-1)+2)+1 = 3U_{n-1}
\end{aligned}
$$

We see that $U_n = 3^n \therefore X_n = 3^n - 1$

## Exercise 3:

We prove it by induction on the amount of discs.
Base case (h = 1):
We start from A, go through C, and finish in B. There is not other possible arrangement than these three.

Inductive hypothesis (h = n):
We pass through all the properly stacked arrangements of the tower of size n, $T_n$.

Proof (h = n+1):
We take $T_n$, and move them to B. By the inductive hypothesis, we pass through all the possible properly stacked arrangements of size n, with the bottom (n+1) disc on A. We move the bottom disc to C, and move $T_n$ to A, once again passing through all the properly stacked arrangements with the bottom disk on C, by the inductive hypothesis. Finally, we move the bottom disk to B, and move $T_n$ back to B, and again by the inductive hypothesis we pass through all the possible properly stacked arrangements of $T_n$.

Recapitulating, we passed through all the properly stacked arrangements of $T_n$ with the bottom disc on A, C, and B. Therefore, we passed through all the properly stacked arrangements of $T_{n+1}$.

## Exercise 4:

Trivially no, since it was proved in the chapter that $T_n = 2^n - 1$, so
whatever amount of moves we need, it is not going to be more than that. In other
words, what the book answers say.

## Exercise 5:

For no circle, we have a single region, i.e. $C_0 = 1$. For a single circle we
have the area inside and outside, so $C_1 = 2$. For the rest:

![$C_2 = 4$](/images/venn21.png)

![$C_3 = 8$](/images/venn31.png)

![$C_4 = 14$](/images/venn41.png)

We would need $C_4$ to be $16$, but that is not the case.
Each circle we add intersects the other circles in two places, creating two regions, meaning we have the following recurrence relation:
$$
\begin{aligned}
C_1 &=2\\
C_n &= C_{n-1} + 2(n-1)
\end{aligned}
$$
If we unfold a couple of terms, we see we can rewrite $C_n$ in closed form:
$$
\begin{aligned}
C_n &= C_{n-1} + 2(n-1)\\
&=C_{n-2} + 2(n-2) + 2(n-1)\\
& \enspace \vdots \\
&=C_1 +2 +4 + \dots + 2(n-2) + 2(n-1) \\
&= C_1+2S_{n-1} = 2 + 2\frac{n(n-1)}{2} = n^2 -n + 2
\end{aligned}
$$

## Exercise 6:

We can easily see that we need at least 3 lines to form an enclosed region, so:
$B_0 = 0, B_1 = 0, B_2 = 0$ From there on, we see a couple more:

![$B_3 = 1$](/images/ch1_ex6_b3.png)

![$B_4 = 3$](/images/ch1_ex6_b4.png)

![$B_5 = 6$](/images/ch1_ex6_b5.png)

![$B_6 = 10$](/images/ch1_ex6_b6.png)

After playing with this, we see that parallel lines are useless. The number of
enclosed regions is a function of the number of distinct points where lines
intersect. If the new line intersects the rest in $k$ points, it generates $(k-1)$
regions. If we had $(n-1)$ lines and add the nth one, we have all the previous
bounded regions, plus at most $(n-2)$ new ones.
Then, we have $B_n = B_{n-1} + (n-2), \forall n \geqslant 2$. If we unfold the
terms, we notice a triangular number sequence, and can rewrite it in closed
form:

$$
\begin{aligned}
B_n &= B_{n-1} + (n-2) \\
&= B_{n-2} + (n-3) + (n-2) \\
& \enspace \vdots \\
&= B_2 + 1 + 2 + \dots + (n-2)\\
&= 0 + S_{n-2} = (n-1)(n-2)/2\\
\end{aligned}
$$

## Exercise 7:

If we try to prove it by induction, we need to start from $n = 1$ (since $J(n)$
is not defined for 0), and we will quickly find that
$H(1) = J(2) - J(1) = 0 \neq 2$
